new/code/github_com/mit_pdos/gokv/asyncfile.v
@@ -169,3 +169,19 @@ Definition MakeAsyncFile : val :=
     let: "$go" := (AsyncFile__flushThread (![ptrT] "s")) in
     do:  (Fork ("$go" #()));;;
     return: (![sliceT] "data", ![ptrT] "s")).
+
+Definition global_id' : string := "github.com/mit-pdos/gokv/asyncfile".
+
+Definition define' : val :=
+  rec: "define'" <> :=
+    exception_do (do:  #()).
+
+Definition initialize' : val :=
+  rec: "initialize'" <> :=
+    exception_do (if: globals.is_uninitialized global_id'
+    then
+      do:  grove_ffi.initialize';;;
+      do:  std.initialize';;;
+      do:  sync.initialize';;;
+      do:  (define' #())
+    else do:  #()).
