new/code/github_com/mit_pdos/gokv/bank.v
@@ -249,4 +249,21 @@ Definition MakeBankClerk : val :=
      let: "$a3" := (![sliceT] "accts") in
      MakeBankClerkSlice "$a0" "$a1" "$a2" "$a3")).
 
+Definition global_id' : string := "github.com/mit-pdos/gokv/bank".
+
+Definition define' : val :=
+  rec: "define'" <> :=
+    exception_do (do:  #()).
+
+Definition initialize' : val :=
+  rec: "initialize'" <> :=
+    exception_do (if: globals.is_uninitialized global_id'
+    then
+      do:  marshal.initialize';;;
+      do:  lockservice.initialize';;;
+      do:  kv.initialize';;;
+      do:  primitive.initialize';;;
+      do:  (define' #())
+    else do:  #()).
+
 End code.
