new/code/github_com/mit_pdos/gokv/reconnectclient.v
@@ -108,3 +108,20 @@ Definition MakeReconnectingClient : val :=
     let: "$r0" := (![uint64T] "addr") in
     do:  ((struct.field_ref ReconnectingClient "addr" (![ptrT] "r")) <-[uint64T] "$r0");;;
     return: (![ptrT] "r")).
+
+Definition global_id' : string := "github.com/mit-pdos/gokv/reconnectclient".
+
+Definition define' : val :=
+  rec: "define'" <> :=
+    exception_do (do:  #()).
+
+Definition initialize' : val :=
+  rec: "initialize'" <> :=
+    exception_do (if: globals.is_uninitialized global_id'
+    then
+      do:  urpc.initialize';;;
+      do:  grove_ffi.initialize';;;
+      do:  primitive.initialize';;;
+      do:  sync.initialize';;;
+      do:  (define' #())
+    else do:  #()).
