new_trusted_code/fmt.v
@@ -7,4 +7,6 @@ Context `{ffi_syntax}.
 Definition Print : val := variadic_noop.
 Definition Printf : val := variadic_noop.
 
+Definition initialize' : val := λ: <>, #().
+
 End code.
