new/proof/globals_test.v
@@ -1,0 +1,24 @@
+From New.proof Require Import grove_prelude.
+From New.code.github_com.mit_pdos.gokv Require globals_test.
+From Perennial.algebra Require Import map.
+From New.proof Require Import std.
+
+Section proof.
+
+Context `{!heapGS Σ}.
+
+Lemma wp_define' :
+  {{{ True }}}
+    globals_test.define' #()
+  {{{ RET #(); True }}}.
+Proof.
+Admitted.
+
+Lemma wp_initialize' :
+  {{{ True }}}
+    globals_test.initialize' #()
+  {{{ RET #(); True }}}.
+Proof.
+Admitted.
+
+End proof.
